Lift qualifier combinators to prelude

ChoiceType/theories/Qualifier.v
@@ -14,72 +14,35 @@ Definition type_qualifier_of {V : Type} `{ValueSig V} : Type :=
 
 Definition type_qualifier : Type := type_qualifier_of (V := value).
 
-Definition tqual {V : Type} `{ValueSig V}
-    (B : gset nat) (d : aset)
-    (prop : gmap nat V → gmap atom V → gmap atom V → Prop) :
-    type_qualifier_of (V := V) :=
-  qual B d prop.
-
 (** ** Locally-nameless infrastructure *)
 
-Definition qual_open {V : Type} `{ValueSig V}
-    (k : nat) (x : atom) (q : type_qualifier_of (V := V)) : type_qualifier_of (V := V) :=
-  qual_open_atom k x q.
-
-Definition qual_open_with_value (k : nat) (v : value) (q : type_qualifier) :
-    type_qualifier :=
-  qual_open_value k v q.
-
-Definition qual_fv {V : Type} `{ValueSig V} (q : type_qualifier_of (V := V)) : aset :=
-  qual_dom q.
-
-Definition qual_subst_one (x : atom) (v : value) (q : type_qualifier) : type_qualifier :=
-  qual_subst_value x v q.
-
-Definition qual_subst (σ : gmap atom value) (q : type_qualifier) : type_qualifier :=
-  qual_subst_map σ q.
-
-#[global] Instance open_qual_inst      : Open value type_qualifier := qual_open_with_value.
-#[global] Instance open_qual_atom_inst : Open atom type_qualifier := qual_open.
-#[global] Instance stale_qual_inst     : Stale type_qualifier := qual_fv.
-#[global] Instance subst_qual_inst     : SubstV value type_qualifier := qual_subst_one.
-#[global] Instance substM_qual_inst    : SubstM (gmap atom value) type_qualifier := qual_subst.
+#[global] Instance open_qual_inst      : Open value type_qualifier := qual_open_value.
+#[global] Instance open_qual_atom_inst : Open atom type_qualifier := qual_open_atom.
+#[global] Instance subst_qual_inst     : SubstV value type_qualifier := qual_subst_value.
+#[global] Instance substM_qual_inst    : SubstM (gmap atom value) type_qualifier := qual_subst_map.
 Arguments open_qual_inst /.
 Arguments open_qual_atom_inst /.
-Arguments stale_qual_inst /.
 Arguments subst_qual_inst /.
 Arguments substM_qual_inst /.
 
-Notation "q '^q^' x" := (qual_open 0 x q) (at level 20).
-Notation "'{' x ':=' v '}q' q" := (qual_subst_one x v q)
+Notation "q '^q^' x" := (qual_open_atom 0 x q) (at level 20).
+Notation "'{' x ':=' v '}q' q" := (qual_subst_value x v q)
   (at level 20, x constr, v constr, format "{ x := v }q  q").
 
 (** ** Local closure *)
-
-Definition lc_qualifier (q : type_qualifier) : Prop :=
-  qual_bvars q = ∅.
 
 #[global] Instance lc_qual_inst : Lc type_qualifier := lc_qualifier.
 Arguments lc_qual_inst /.
 
 (** ** Conjunction of two shallow qualifiers *)
 
-Definition qualifier_and (q1 q2 : type_qualifier) : type_qualifier :=
-  match q1, q2 with
-  | qual B1 d1 prop1, qual B2 d2 prop2 =>
-      qual (B1 ∪ B2) (d1 ∪ d2) (fun β σ ρ => prop1 β σ ρ ∧ prop2 β σ ρ)
-  end.
-
-Notation "q1 '&q' q2" := (qualifier_and q1 q2) (at level 40).
+Notation "q1 '&q' q2" := (qual_and q1 q2) (at level 40).
 
 (** ** Denotation helpers *)
 
 Definition qual_interp_full
     (β : gmap nat value) (σ ρ : gmap atom value) (q : type_qualifier) : Prop :=
-  match q with
-  | qual B d prop =>
-      prop (map_restrict value β B) (store_restrict σ d) (store_restrict ρ d)
-  end.
+  qual_denote_with (λ d ρ, store_restrict ρ d) q β σ ρ.
 
 Definition qual_interp (σ : gmap atom value) (q : type_qualifier) : Prop :=
   qual_interp_full ∅ σ σ q.
@@ -132,8 +95,6 @@ Notation "'b0:x=' x" := (mk_q_eq (vbvar 0) (vfvar x))
 Notation "'b0:c=' c" := (mk_q_eq (vbvar 0) (vconst c))
   (at level 5, format "b0:c= c").
 
-Definition qual_top : type_qualifier := qual ∅ ∅ (fun _ _ _ => True).
-Definition qual_bot : type_qualifier := qual ∅ ∅ (fun _ _ _ => False).
 Notation "⊤q" := qual_top.
 Notation "⊥q" := qual_bot.
 
@@ -153,7 +114,7 @@ Proof. Admitted.
 
 Lemma qual_interp_subst_compose (σ_X σ : gmap atom value) (q : type_qualifier) :
   store_compat σ_X σ →
-  qual_interp σ (qual_subst σ_X q) ↔ qual_interp (σ_X ∪ σ) q.
+  qual_interp σ (qual_subst_map σ_X q) ↔ qual_interp (σ_X ∪ σ) q.
 Proof. Admitted.
 
 Lemma qual_interp_and q1 q2 σ :
